agree/stateScript.sml
@@ -1,0 +1,191 @@
+open HolKernel Parse boolLib bossLib BasicProvers
+     pred_setLib stringLib intLib finite_mapTheory
+     arithmeticTheory listTheory pred_setTheory
+     agreeTheory;
+
+val _ = intLib.prefer_int();
+
+val _ = new_theory "state";
+
+(*---------------------------------------------------------------------------*)
+(* Conventional notion of state, mapping from name to value. NB: since we    *)
+(* are defining step-wise computation, the temporal operators Pre, Fby, and  *)
+(* Hist are treated differently. Pre is treated as the identity function,    *)
+(* and Fby is treated as a test on an implicit "_initStep" boolean stream,   *)
+(* while Hist is not allowed in the syntax.                                  *)
+(*---------------------------------------------------------------------------*)
+
+Type value_env = “:string |-> value”
+
+Definition updateState_def :
+ updateState (fmap:value_env) name value = fmap |+ (name,value)
+End
+
+(*---------------------------------------------------------------------------*)
+(* Map stream env to state                                                   *)
+(*---------------------------------------------------------------------------*)
+
+Definition strmIndex_def:
+  strmIndex (E:string |-> (num -> value)) t = FMAP_MAP2 (\(s,strm). strm t) E
+End
+
+(*---------------------------------------------------------------------------*)
+(* Custom size for expressions used in termination proof of evalue/bvalue    *)
+(*---------------------------------------------------------------------------*)
+
+Definition expr_sizeA_def :
+  expr_sizeA (IntVar s) = 0n /\
+  expr_sizeA (IntLit i) = 0  /\
+  expr_sizeA (AddExpr e1 e2)  = 1 + expr_sizeA e1 + expr_sizeA e2 /\
+  expr_sizeA (SubExpr e1 e2)  = 1 + expr_sizeA e1 + expr_sizeA e2 /\
+  expr_sizeA (MultExpr e1 e2) = 1 + expr_sizeA e1 + expr_sizeA e2 /\
+  expr_sizeA (DivExpr e1 e2)  = 1 + expr_sizeA e1 + expr_sizeA e2 /\
+  expr_sizeA (ModExpr e1 e2)  = 1 + expr_sizeA e1 + expr_sizeA e2 /\
+  expr_sizeA (CondExpr b x y) = 1 + bexpr_sizeA b + expr_sizeA x + expr_sizeA y   /\
+  expr_sizeA (FbyExpr e1 e2)  = 1 + expr_sizeA e1 + expr_sizeA e2 /\
+  expr_sizeA (PreExpr e)      = 1 + expr_sizeA e
+  ∧
+  bexpr_sizeA (BoolVar s)     = 0n /\
+  bexpr_sizeA (BoolLit b)     = 0  /\
+  bexpr_sizeA (NotExpr b)     = 1 + bexpr_sizeA b /\
+  bexpr_sizeA (OrExpr b1 b2)  = 1 + bexpr_sizeA b1 + bexpr_sizeA b2 /\
+  bexpr_sizeA (AndExpr b1 b2) = 1 + bexpr_sizeA b1 + bexpr_sizeA b2 /\
+  bexpr_sizeA (ImpExpr b1 b2) = 1 + bexpr_sizeA b1 + bexpr_sizeA b2 /\
+  bexpr_sizeA (IffExpr b1 b2) = 1 + bexpr_sizeA b1 + bexpr_sizeA b2 /\
+  bexpr_sizeA (EqExpr e1 e2)  = 1 + expr_sizeA e1 + expr_sizeA e2 /\
+  bexpr_sizeA (LtExpr e1 e2)  = 1 + expr_sizeA e1 + expr_sizeA e2 /\
+  bexpr_sizeA (LeqExpr e1 e2) = 1 + expr_sizeA e1 + expr_sizeA e2 /\
+  bexpr_sizeA (BoolCondExpr b b1 b2) = 1 + bexpr_sizeA b + bexpr_sizeA b1 + bexpr_sizeA b2 /\
+  bexpr_sizeA (BoolFbyExpr b1 b2)    = 1 + bexpr_sizeA b1 + bexpr_sizeA b2 /\
+  bexpr_sizeA (BoolPreExpr b) = 1 + bexpr_sizeA b /\
+  bexpr_sizeA (HistExpr b)    = 0
+End
+
+Definition evalue_def :
+  evalue E (IntVar s) = int_of (E ' s) /\
+  evalue E (IntLit i) = i /\
+  evalue E (AddExpr e1 e2)  = evalue E e1 + evalue E e2  /\
+  evalue E (SubExpr e1 e2)  = evalue E e1 - evalue E e2  /\
+  evalue E (MultExpr e1 e2) = evalue E e1 * evalue E e2 /\
+  evalue E (DivExpr e1 e2)  = evalue E e1 / evalue E e2  /\
+  evalue E (ModExpr e1 e2)  = evalue E e1 % evalue E e2  /\
+  evalue E (CondExpr b e1 e2) = (if bvalue E b then evalue E e1 else evalue E e2) ∧
+  evalue E (PreExpr e)      = evalue E e /\
+  evalue E (FbyExpr e1 e2)  =
+      (if bvalue E (BoolVar "_initStep") then evalue E e1 else evalue E e2)
+  /\
+  bvalue E (BoolVar s)     = bool_of (E ' s) /\
+  bvalue E (BoolLit b)     = b /\
+  bvalue E (NotExpr b)     = (~bvalue E b) /\
+  bvalue E (OrExpr b1 b2)  = (bvalue E b1 \/ bvalue E b2) /\
+  bvalue E (AndExpr b1 b2) = (bvalue E b1 /\ bvalue E b2) /\
+  bvalue E (ImpExpr b1 b2) = (bvalue E b1 ⇒ bvalue E b2) /\
+  bvalue E (IffExpr b1 b2) = (bvalue E b1 = bvalue E b2) /\
+  bvalue E (EqExpr e1 e2)  = (evalue E e1 = evalue E e2)   /\
+  bvalue E (LtExpr e1 e2)  = (evalue E e1 < evalue E e2)   /\
+  bvalue E (LeqExpr e1 e2) = (evalue E e1 <= evalue E e2)  /\
+  bvalue E (BoolCondExpr b b1 b2) = (if bvalue E b then bvalue E b1 else bvalue E b2) ∧
+  bvalue E (BoolPreExpr b) = bvalue E b /\
+  bvalue E (BoolFbyExpr b1 b2) =
+      (if bvalue E (BoolVar "_initStep") then bvalue E b1 else bvalue E b2) ∧
+  bvalue E (HistExpr b)    = ARB
+Termination
+  WF_REL_TAC ‘measure (sum_size (expr_sizeA o SND) (bexpr_sizeA o SND))’
+  >> rw [expr_sizeA_def]
+End
+
+(*---------------------------------------------------------------------------*)
+(* Meaning of variable definitions                                           *)
+(*---------------------------------------------------------------------------*)
+
+Definition defFn_def :
+ defFn E (IntStmt s exp)   = updateState E s (IntValue(evalue E exp)) ∧
+ defFn E (BoolStmt s bexp) = updateState E s (BoolValue(bvalue E bexp))
+End
+
+(*---------------------------------------------------------------------------*)
+(* Sequential accumulation of variable updates.                              *)
+(*---------------------------------------------------------------------------*)
+
+Definition defListFn_def : defListFn E defs = FOLDL defFn E defs
+End
+
+(*---------------------------------------------------------------------------*)
+(* Given inputs and a state, produce the new state and outputs               *)
+(*                                                                           *)
+(*   stateStep: component -> inputs # state -> state # outputs               *)
+(*                                                                           *)
+(* where inputs, state, and outputs are value environments (string |-> value)*)
+(*---------------------------------------------------------------------------*)
+
+Definition stateStep_def :
+  stateStep comp (inE,stateE) =
+  let E = FUNION inE stateE ;
+      E' = defListFn E (comp.var_defs ++ comp.out_defs) ;
+      stateE' = DRESTRICT E' (set (MAP defName comp.var_defs)) ;
+      outE    = DRESTRICT E' (set (MAP defName comp.out_defs))
+  in (stateE', outE)
+End
+
+Definition stateSteps_def :
+  stateSteps inputs init comp 0 = stateStep comp (strmIndex inputs 0,init) ∧
+  stateSteps inputs init comp (SUC t) =
+     let (stateE,outE) = stateSteps inputs init comp t
+     in stateStep comp (strmIndex inputs (SUC t),stateE)
+End
+
+(*---------------------------------------------------------------------------*)
+(* Running the state stepper for t steps gives the same answers as running   *)
+(* the stream stepper for t steps and looking at the (state,output) just at  *)
+(* time t.                                                                   *)
+(*                                                                           *)
+(* This statement is only true if comp is in a form where it looks back at   *)
+(* most one step in its history. And comp has to be wellformed and env has   *)
+(* to support it, as in agreeTheory.                                         *)
+(*---------------------------------------------------------------------------*)
+
+Theorem stepper_equiv :
+  ∀E init comp t result.
+     Wellformed comp ∧ Supports E comp ∧
+     result = strmIndex (strmSteps E comp t) t
+     ⇒
+     stateSteps (input_of comp E) init comp t =
+     (state_of comp result,output_of comp result)
+Proof
+  cheat
+(*
+  Induct_on ‘t’
+  >- rw[stateSteps_def,strmSteps_def,stateStep_def,strmStep_def]
+*)
+QED
+
+Definition fmap_map_def:
+ fmap_map f = FMAP_MAP2 (\(d,r). f r)
+End
+
+(*---------------------------------------------------------------------------*)
+(* Given inputs and a state, produce the new state and outputs               *)
+(*                                                                           *)
+(*  bufStep: component -> inputs # state -> state # outputs                  *)
+(*                                                                           *)
+(* where state is a (string |-> value) environment and inputs/outputs are    *)
+(* (string |-> string) environments. This models the use of byte buffers for *)
+(* component input and output. For now assume the existence of suitable      *)
+(* encoders and decoders (enc,dec).                                          *)
+(*---------------------------------------------------------------------------*)
+
+Type buf_env = “:string |-> string”
+
+Definition bufStep_def:
+  bufStep (enc:value->string,dec:string->value) comp (inE,stateE) =
+    let inputs = fmap_map dec inE;
+        (stateE',outE) = stateStep comp (inputs,stateE);
+        outE' = fmap_map enc outE;
+    in (stateE',outE')
+End
+
+val _ = TeX_notation {hol = "FUNION",        TeX = ("\\HOLTokenFmapUnion", 1)};
+val _ = TeX_notation {hol = UTF8.chr 0x228C, TeX = ("\\HOLTokenFmapUnion", 1)};
+val _ = TeX_notation {hol = "fmap_map", TeX = ("fmap\\_map", 8)};
+
+val _ = export_theory();
