agree/stepScript.sml
@@ -1,0 +1,129 @@
+open HolKernel Parse boolLib bossLib BasicProvers
+     pred_setLib stringLib intLib finite_mapTheory
+     arithmeticTheory listTheory pred_setTheory
+     agreeTheory;
+
+val _ = intLib.prefer_int();
+
+val _ = new_theory "step";
+
+(*---------------------------------------------------------------------------*)
+(* Conventional state, mapping from name to value. Also evaluation.          *)
+(* NB: since we are defining step-wise computation, the temporal operators   *)
+(* Pre, Fby, and Hist are treated differently. Pre is treated as the identity*)
+(* function, and Fby/Hist is not allowed in the syntax. We handle this by    *)
+(* putting ARB for the semantic value.                                       *)
+(*---------------------------------------------------------------------------*)
+
+Type state = “:string |-> value”
+
+Definition updateState_def :
+ updateState (fmap:state) name value = fmap |+ (name,value)
+End
+
+(*---------------------------------------------------------------------------*)
+(* Custom size for expressions used in termination proof of evalue/bvalue    *)
+(*---------------------------------------------------------------------------*)
+
+Definition expr_sizeA_def :
+  expr_sizeA (IntVar s) = 0n /\
+  expr_sizeA (IntLit i) = 0  /\
+  expr_sizeA (AddExpr e1 e2)  = 1 + expr_sizeA e1 + expr_sizeA e2 /\
+  expr_sizeA (SubExpr e1 e2)  = 1 + expr_sizeA e1 + expr_sizeA e2 /\
+  expr_sizeA (MultExpr e1 e2) = 1 + expr_sizeA e1 + expr_sizeA e2 /\
+  expr_sizeA (DivExpr e1 e2)  = 1 + expr_sizeA e1 + expr_sizeA e2 /\
+  expr_sizeA (ModExpr e1 e2)  = 1 + expr_sizeA e1 + expr_sizeA e2 /\
+  expr_sizeA (CondExpr b x y) = 1 + bexpr_sizeA b + expr_sizeA x + expr_sizeA y   /\
+  expr_sizeA (FbyExpr e1 e2)  = 1 + expr_sizeA e1 + expr_sizeA e2 /\
+  expr_sizeA (PreExpr e)      = 1 + expr_sizeA e
+  ∧
+  bexpr_sizeA (BoolVar s)     = 0n /\
+  bexpr_sizeA (BoolLit b)     = 0  /\
+  bexpr_sizeA (NotExpr b)     = 1 + bexpr_sizeA b /\
+  bexpr_sizeA (OrExpr b1 b2)  = 1 + bexpr_sizeA b1 + bexpr_sizeA b2 /\
+  bexpr_sizeA (AndExpr b1 b2) = 1 + bexpr_sizeA b1 + bexpr_sizeA b2 /\
+  bexpr_sizeA (ImpExpr b1 b2) = 1 + bexpr_sizeA b1 + bexpr_sizeA b2 /\
+  bexpr_sizeA (IffExpr b1 b2) = 1 + bexpr_sizeA b1 + bexpr_sizeA b2 /\
+  bexpr_sizeA (EqExpr e1 e2)  = 1 + expr_sizeA e1 + expr_sizeA e2 /\
+  bexpr_sizeA (LtExpr e1 e2)  = 1 + expr_sizeA e1 + expr_sizeA e2 /\
+  bexpr_sizeA (LeqExpr e1 e2) = 1 + expr_sizeA e1 + expr_sizeA e2 /\
+  bexpr_sizeA (BoolCondExpr b b1 b2) = 1 + bexpr_sizeA b + bexpr_sizeA b1 + bexpr_sizeA b2 /\
+  bexpr_sizeA (BoolFbyExpr b1 b2)    = 1 + bexpr_sizeA b1 + bexpr_sizeA b2 /\
+  bexpr_sizeA (BoolPreExpr b) = 1 + bexpr_sizeA b /\
+  bexpr_sizeA (HistExpr b)    = 0
+End
+
+Definition evalue_def :
+  evalue E (IntVar s) = int_of (E ' s) /\
+  evalue E (IntLit i) = i /\
+  evalue E (AddExpr e1 e2)  = evalue E e1 + evalue E e2  /\
+  evalue E (SubExpr e1 e2)  = evalue E e1 - evalue E e2  /\
+  evalue E (MultExpr e1 e2) = evalue E e1 * evalue E e2 /\
+  evalue E (DivExpr e1 e2)  = evalue E e1 / evalue E e2  /\
+  evalue E (ModExpr e1 e2)  = evalue E e1 % evalue E e2  /\
+  evalue E (CondExpr b e1 e2) = (if bvalue E b then evalue E e1 else evalue E e2) ∧
+  evalue E (PreExpr e)      = evalue E e /\
+  evalue E (FbyExpr e1 e2)  =
+      (if bvalue E (BoolVar "_initStep") then evalue E e1 else evalue E e2)
+  /\
+  bvalue E (BoolVar s)     = bool_of (E ' s) /\
+  bvalue E (BoolLit b)     = b /\
+  bvalue E (NotExpr b)     = (~bvalue E b) /\
+  bvalue E (OrExpr b1 b2)  = (bvalue E b1 \/ bvalue E b2) /\
+  bvalue E (AndExpr b1 b2) = (bvalue E b1 /\ bvalue E b2) /\
+  bvalue E (ImpExpr b1 b2) = (bvalue E b1 ⇒ bvalue E b2) /\
+  bvalue E (IffExpr b1 b2) = (bvalue E b1 = bvalue E b2) /\
+  bvalue E (EqExpr e1 e2)  = (evalue E e1 = evalue E e2)   /\
+  bvalue E (LtExpr e1 e2)  = (evalue E e1 < evalue E e2)   /\
+  bvalue E (LeqExpr e1 e2) = (evalue E e1 <= evalue E e2)  /\
+  bvalue E (BoolCondExpr b b1 b2) = (if bvalue E b then bvalue E b1 else bvalue E b2) ∧
+  bvalue E (BoolPreExpr b) = bvalue E b /\
+  bvalue E (BoolFbyExpr b1 b2) =
+      (if bvalue E (BoolVar "_initStep") then bvalue E b1 else bvalue E b2) ∧
+  bvalue E (HistExpr b)    = ARB
+Termination
+  WF_REL_TAC ‘measure (sum_size (expr_sizeA o SND) (bexpr_sizeA o SND))’
+  >> rw [expr_sizeA_def]
+End
+
+Definition defFn_def :
+ defFn E (IntStmt s exp)   = updateState E s (IntValue(evalue E exp)) ∧
+ defFn E (BoolStmt s bexp) = updateState E s (BoolValue(bvalue E bexp))
+End
+
+(*---------------------------------------------------------------------------*)
+(* Sequential accumulation of variable updates.                              *)
+(*---------------------------------------------------------------------------*)
+
+Definition defListFn_def : defListFn E defs = FOLDL defFn E defs
+End
+
+(*---------------------------------------------------------------------------*)
+(* Given inputs and a state, produce the new state and outputs               *)
+(*                                                                           *)
+(*   stateStep: component -> inputs # state -> state # outputs               *)
+(*                                                                           *)
+(* where inputs, state, and outputs are environments (string |-> value)      *)
+(*---------------------------------------------------------------------------*)
+
+Definition stateStep_def :
+  stateFn comp (inE,stateE) =
+  let E = FUNION inE stateE ;
+      E' = defListFn E (comp.var_defs ++ comp.out_defs) ;
+      stateE' = DRESTRICT E' (set (MAP defName comp.var_defs)) ;
+      outE    = DRESTRICT E' (set (MAP defName comp.out_defs))
+  in (stateE', outE)
+End
+
+
+(*---------------------------------------------------------------------------*)
+(*
+(*---------------------------------------------------------------------------*)
+
+Theorem
+ ∀
+Proof
+QED
+*)
+
+val _ = export_theory();
